$$ x^{2} y^{2} y' +1=y $$
$$ \int \dfrac{y^2}{y-1} dx=\int \dfrac{dx}{x^2} $$ 
$$ x^{2} y^{2} dy=(y-1)dx $$
$$ x^{2} y^{2} \dfrac{dy}{dx}=y-1 $$
$$y'=f(x)g(y)$$

$$ x^{2} y'' -4xy'+6y=0 $$
$$ x^{2} y'' -2y=\sin \ln(x) $$
$$y_1=e^{2x}\cos x $$

$$  \begin{cases}
    \dot{x}=2y-x+1\\
    \dot{y}=3y-2x
\end{cases}$$ 

$$  \begin{cases}
    \dot{x}=2x-y\\
    \dot{y}=x+2e^{t}
\end{cases}$$ 

$$\dot{x}=Ax,A=\begin{pmatrix}
3 & 0 \\ 
 0 & 3\\ 
\end{pmatrix}$$ 

$$\dot{x}=Ax,A=\begin{pmatrix}
-1& -2 & 2 \\ 
 -2& -1 & 2\\ 
 -3& -2 & 3\\ 
\end{pmatrix}$$ 